Primitives (#747)
* Quotation of the retroknowledge info, add support for int and float

* Adapt PCUIC to new typing rule for primitive values

* Adapted safe checker and erasure to retroknowledge/primitive types

* Adapted examples

* Fixups

* Add ind_finite field to mutual inductives and fix CoFix quoting in extracted code

* Fix todo, add primitive typing rule to Template typing

* Fix .mlpack for compatibility with ocaml 4.07

template-coq/src/denoter.ml
@@ -158,8 +158,8 @@ struct
          let p' = Names.Projection.make p' false in
          let evm, t' = aux env evm t in
          evm, Constr.mkProj (p', t')
-      (* | ACoq_tInt x -> evm, Constr.mkInt (D.unquote_int63 x) *)
-      (* | ACoq_tFloat x -> evm, Constr.mkFloat (D.unquote_float64 x) *)
+      | ACoq_tInt x -> evm, Constr.mkInt (D.unquote_int63 x)
+      | ACoq_tFloat x -> evm, Constr.mkFloat (D.unquote_float64 x)
 
     in aux env evm trm
 
