erasure/theories/ELiftSubst.v
@@ -35,7 +35,7 @@ Fixpoint lift n k t : term :=
   | tVar _ => t
   | tConst _ => t
   | tConstruct ind i args => tConstruct ind i (map (lift n k) args)
-  (* | tPrim _ => t *)
+  | tPrim _ => t
   end.
 
 Notation lift0 n := (lift n 0).
