safechecker/theories/PCUICEqualityDec.v
@@ -157,7 +157,7 @@ Fixpoint eqb_term_upto_univ_napp
       eqb_binder_annot x.(dname) y.(dname)
     ) mfix mfix'
 
-(*  | tPrim p, tPrim p' => eqb p p' *)
+  | tPrim p, tPrim p' => eqb p p'
 
   | _, _ => false
   end.
@@ -740,7 +740,7 @@ Proof.
         constructor. constructor. constructor ; try easy.
         now inversion e3.
 
-(*  - cbn - [eqb]. eqspecs. do 2 constructor. *)
+ - cbn - [eqb]. eqspecs. do 2 constructor.
 Qed.
 
  Lemma eqb_term_upto_univ_impl (equ lequ : _ -> _ -> bool)
