safechecker/theories/PCUICSafeConversion.v
@@ -5143,7 +5143,7 @@ Qed.
     - reflexivity.
   Qed.
 
-  (* TODO move to PCUICNormal
+  (* TODO move to PCUICNormal *)
   Lemma whnf_mkApps_tPrim_inv : 
     forall (f : RedFlags.t) (Σ : global_env) (Γ : context) p (args : list term),
       whnf f Σ Γ (mkApps (tPrim p) args) -> args = [].
@@ -5159,7 +5159,7 @@ Qed.
     rewrite mkApps_app in teq.
     cbn in teq. noconf teq.
     eauto.
-  Qed. *)
+  Qed.
 
   Lemma reducible_head_None Σ (wfΣ : abstract_env_ext_rel X Σ) Γ t π h :
     isApp t = false ->
@@ -5219,9 +5219,9 @@ Qed.
     - constructor; eexists _, (decompose_stack π).1.
       split; [constructor; eauto with pcuic|].
       eauto with pcuic.
-(*    - apply whnf_mkApps_tPrim_inv in wh as ->.
+    - apply whnf_mkApps_tPrim_inv in wh as ->.
       constructor; eexists _, [].
-      eauto using whnf_red with pcuic.*)
+      eauto using whnf_red with pcuic.
     - constructor; eexists _, (decompose_stack π).1.
       clear H. erewrite <- abstract_env_lookup_correct in e; eauto. 
       split; [econstructor|]; eauto.
